src/cbor/pulse/raw/everparse/CBOR.Pulse.Raw.Format.Parse.fst
@@ -391,7 +391,7 @@ fn cbor_raw_sorted (sq: squash SZ.fits_u64) : LowParse.Pulse.Recursive.impl_pred
     )
     a #pm v'
   );
-  let Mktuple2 input1 input2 = split_nondep_then_tot_kind serialize_header (jump_header ()) // FIXME: WHY WHY WHY do the kinds need to be total here?
+  let input1, input2 = split_nondep_then_tot_kind serialize_header (jump_header ()) // FIXME: WHY WHY WHY do the kinds need to be total here?
       (LowParse.Spec.Combinators.serialize_nondep_then
         (serialize_leaf_content gh)
         (LowParse.Pulse.Recursive.serialize_nlist_recursive_cons_payload serialize_raw_data_item_param (SZ.v n) l)
@@ -403,7 +403,7 @@ fn cbor_raw_sorted (sq: squash SZ.fits_u64) : LowParse.Pulse.Recursive.impl_pred
         (serialize_leaf_content gh)
         (LowParse.Pulse.Recursive.serialize_nlist_recursive_cons_payload serialize_raw_data_item_param (SZ.v n) l)
       )
-      a pm v' (Mktuple2 input1 input2)
+      a pm v' (input1, input2)
   );
   unfold (split_nondep_then_post'
     serialize_header
@@ -443,7 +443,7 @@ fn cbor_raw_sorted (sq: squash SZ.fits_u64) : LowParse.Pulse.Recursive.impl_pred
         )
         input3;
       Trade.trans _ _ (pts_to_serialized (LowParse.Spec.VCList.serialize_nlist (SZ.v n) (serializer_of_tot_serializer (LowParse.Spec.Recursive.serialize_recursive serialize_raw_data_item_param))) a #pm va);
-      let Mktuple2 hd4 input4 = LowParse.Pulse.VCList.nlist_hd_tl_nondep_then_left
+      let hd4, input4 = LowParse.Pulse.VCList.nlist_hd_tl_nondep_then_left
         serialize_raw_data_item
         ()
         (jump_raw_data_item ())
@@ -494,7 +494,7 @@ fn cbor_raw_sorted (sq: squash SZ.fits_u64) : LowParse.Pulse.Recursive.impl_pred
           (pts_to_serialized (serialize_nondep_then (LowParse.Spec.VCList.serialize_nlist vn serialize_raw_data_item) s) stail #pm vtail)
           (pts_to_serialized (serialize_nondep_then (LowParse.Spec.VCList.serialize_nlist vn serialize_raw_data_item) s) tail #pm vtail);
         Trade.trans_hyp_r _ _ _ (pts_to_serialized (LowParse.Spec.VCList.serialize_nlist (SZ.v n) (serializer_of_tot_serializer (LowParse.Spec.Recursive.serialize_recursive serialize_raw_data_item_param))) a #pm va);
-        let Mktuple2 key2 tail2 = LowParse.Pulse.VCList.nlist_hd_tl_nondep_then_left serialize_raw_data_item () (jump_raw_data_item ()) vn () s tail;
+        let key2, tail2 = LowParse.Pulse.VCList.nlist_hd_tl_nondep_then_left serialize_raw_data_item () (jump_raw_data_item ()) vn () s tail;
         let key1 = !pkey;
         let res = impl_deterministically_encoded_cbor_map_key_order () key1 key2;
         if res {
