src/lowparse/pulse/LowParse.Pulse.Base.fst
@@ -414,19 +414,15 @@ fn peek
   returns res: (slice byte & slice byte)
   ensures peek_post s input pm v consumed res
 {
-  let s1s2 = split input consumed;
-  match s1s2 {
-    Mktuple2 s1 s2 -> {
-      Seq.lemma_split v (SZ.v consumed);
-      let v1 = Ghost.hide (fst (Some?.v (parse p v)));
-      parse_injective #k p (bare_serialize s v1) v;
-      with v1' . assert (pts_to s1 #pm v1');
-      rewrite (pts_to s1 #pm v1') as (pts_to_serialized s s1 #pm v1);
-      fold (peek_post' s input pm v consumed s1 s2);
-      fold (peek_post s input pm v consumed (s1, s2));
-      (s1, s2)
-    }
-  }
+  let s1, s2 = split input consumed;
+  Seq.lemma_split v (SZ.v consumed);
+  let v1 = Ghost.hide (fst (Some?.v (parse p v)));
+  parse_injective #k p (bare_serialize s v1) v;
+  with v1' . assert (pts_to s1 #pm v1');
+  rewrite (pts_to s1 #pm v1') as (pts_to_serialized s s1 #pm v1);
+  fold (peek_post' s input pm v consumed s1 s2);
+  fold (peek_post s input pm v consumed (s1, s2));
+  (s1, s2)
 }
 
 let peek_trade_post'
@@ -489,16 +485,14 @@ fn peek_trade
   returns res: (slice byte & slice byte)
   ensures peek_trade_post s input pm v consumed res
 {
-  let res = peek s input consumed;
-  match res { Mktuple2 left right -> {
-    unfold (peek_post s input pm v consumed res);
-    unfold (peek_post' s input pm v consumed left right);
-    with v1 v2 . assert (pts_to_serialized s left #pm v1 ** pts_to right #pm v2);
-    intro_trade (pts_to_serialized s left #pm v1 ** pts_to right #pm v2) (pts_to input #pm v) (is_split input left right) (peek_trade_aux s input pm consumed v left right v1 v2 ());
-    fold (peek_trade_post' s input pm v consumed left right);
-    fold (peek_trade_post s input pm v consumed (left, right));
-    (left, right)
-  }}
+  let left, right = peek s input consumed;
+  unfold (peek_post s input pm v consumed (left, right));
+  unfold (peek_post' s input pm v consumed left right);
+  with v1 v2 . assert (pts_to_serialized s left #pm v1 ** pts_to right #pm v2);
+  intro_trade (pts_to_serialized s left #pm v1 ** pts_to right #pm v2) (pts_to input #pm v) (is_split input left right) (peek_trade_aux s input pm consumed v left right v1 v2 ());
+  fold (peek_trade_post' s input pm v consumed left right);
+  fold (peek_trade_post s input pm v consumed (left, right));
+  (left, right)
 }
 
 inline_for_extraction
@@ -516,21 +510,17 @@ fn peek_trade_gen
     parse p (Seq.slice v (SZ.v offset) (Seq.length v)) == Some (v', SZ.v off - SZ.v offset)
   )
 {
-  let split123 = split_trade input offset;
-  match split123 { Mktuple2 input1 input23 -> {
-    with v23 . assert (pts_to input23 #pm v23);
-    Trade.elim_hyp_l (pts_to input1 #pm _) (pts_to input23 #pm v23) _;
-    let consumed = SZ.sub off offset;
-    let split23 = peek_trade s input23 consumed;
-    match split23 { Mktuple2 input2 input3 -> {
-      unfold (peek_trade_post s input23 pm v23 consumed split23);
-      unfold (peek_trade_post' s input23 pm v23 consumed input2 input3);
-      with v' . assert (pts_to_serialized s input2 #pm v');
-      Trade.elim_hyp_r (pts_to_serialized s input2 #pm _) (pts_to input3 #pm _) (pts_to input23 #pm v23);
-      Trade.trans (pts_to_serialized s input2 #pm _) (pts_to input23 #pm _) (pts_to input #pm _);
-      input2
-    }}
-  }}
+  let input1, input23 = split_trade input offset;
+  with v23 . assert (pts_to input23 #pm v23);
+  Trade.elim_hyp_l (pts_to input1 #pm _) (pts_to input23 #pm v23) _;
+  let consumed = SZ.sub off offset;
+  let input2, input3 = peek_trade s input23 consumed;
+  unfold (peek_trade_post s input23 pm v23 consumed (input2, input3));
+  unfold (peek_trade_post' s input23 pm v23 consumed input2 input3);
+  with v' . assert (pts_to_serialized s input2 #pm v');
+  Trade.elim_hyp_r (pts_to_serialized s input2 #pm _) (pts_to input3 #pm _) (pts_to input23 #pm v23);
+  Trade.trans (pts_to_serialized s input2 #pm _) (pts_to input23 #pm _) (pts_to input #pm _);
+  input2
 }
 
 inline_for_extraction
@@ -1558,23 +1548,15 @@ fn l2r_write_copy
   S.pts_to_len out;
   S.pts_to_len x.v;
   let length = S.len x.v;
-  let sp1 = S.split out offset;
-  match sp1 {
-    Mktuple2 sp11 sp12 -> {
-      with v12 . assert (pts_to sp12 v12);
-      let sp2 = S.split sp12 length;
-      match sp2 {
-        Mktuple2 sp21 sp22 -> {
-          S.pts_to_len sp21;
-          S.copy sp21 x.v;
-          S.join sp21 sp22 sp12;
-          S.join sp11 sp12 out;
-          Trade.elim _ _;
-          SZ.add offset length;
-        }
-      }
-    }
-  }
+  let sp11, sp12 = S.split out offset;
+  with v12 . assert (pts_to sp12 v12);
+  let sp21, sp22 = S.split sp12 length;
+  S.pts_to_len sp21;
+  S.copy sp21 x.v;
+  S.join sp21 sp22 sp12;
+  S.join sp11 sp12 out;
+  Trade.elim _ _;
+  SZ.add offset length;
 }
 
 inline_for_extraction
